

1. Prove  $\forall x, y, z \in \mathbb{Z}$ , if  $x$  divides  $y$  and  $y$  divides  $z$ , then  $x$  divides  $z$ .

*Proof.*

Let  $x, y, z \in \mathbb{Z}$ .

Assume  $x$  divides  $y$  and  $y$  divides  $z$ .

Let  $a, b \in \mathbb{Z}$  with  $y = ax$  and  $z = by$ .

Let  $c = ab$ .

$$z = by = b(ax) = cx.$$

Therefore,  $\exists c \in \mathbb{Z}$ ,  $z = cx$ . i.e.,  $x$  divides  $z$ .

Therefore, if  $x$  divides  $y$  and  $y$  divides  $z$ , then  $x$  divides  $z$ .

QED

□

2. Prove  $\forall x, y \in \mathbb{Z}$ , if  $xy$  is even and  $y$  is odd, then  $x + y$  is odd.

*Proof.*

Let  $x, y \in \mathbb{Z}$ .

Assume  $xy$  is even and  $y$  is odd.

Let  $a, b \in \mathbb{Z}$  with  $xy = 2a$  and  $y = 2b + 1$ .

Let  $c = a - bx + b$ .

$$2a = xy = x(2b + 1) = 2bx + x, \text{ and so } x = 2a - 2bx.$$

$$\text{Then } x + y = 2a - 2bx + 2b + 1 = 2(a - bx + b) + 1 = 2c + 1.$$

Therefore,  $\exists c \in \mathbb{Z}$ ,  $x + y = 2c + 1$ . i.e.,  $x + y$  is odd.

Therefore, if  $xy$  is even and  $y$  is odd, then  $x + y$  is odd.

QED

□

3. Prove  $\forall x, y \in \mathbb{Z}$ , if  $x + y$  is odd, then  $x - y$  is odd.

*Proof.*

Let  $x, y \in \mathbb{Z}$ . Assume  $x + y$  is odd.

Let  $a \in \mathbb{Z}$  with  $x + y = 2a + 1$ .

Let  $b = a - y$ .

$$x - y = x + y - 2y = 2a + 1 - 2y = 2(a - y) + 1 = 2b + 1.$$

Therefore,  $x - y$  is odd.

Therefore, if  $x + y$  is odd, then  $x - y$  is odd.

QED

□

4. Prove  $\forall x, y \in \mathbb{Z}$ , if 3 divides  $xy$  and 3 divides  $y - 1$ , then 3 divides  $x$ .

*Proof.*

Let  $x, y \in \mathbb{Z}$ .

Assume 3 divides  $xy$  and 3 divides  $y - 1$ .

Let  $a, b \in \mathbb{Z}$  with  $xy = 3a$  and  $y - 1 = 3b$ .

Let  $c = a - xb$ .

$$x = xy - xy + x = xy - x(y - 1) = 3a - x(3b) = 3(a - xb) = 3c.$$

Therefore,  $\exists c \in \mathbb{Z}$ ,  $x = 3c$ . i.e., 3 divides  $x$ .

Therefore, if 3 divides  $xy$  and 3 divides  $y - 1$ , then 3 divides  $x$ .

QED

□

5. Prove  $\forall x \in \mathbb{Z}$ , if 2 divides  $x$  and 5 divides  $x$ , then 10 divides  $x$ .

*Proof.*

Let  $x \in \mathbb{Z}$ .

Assume 2 divides  $x$  and 5 divides  $x$ .

Let  $a, b \in \mathbb{Z}$  with  $x = 2a$  and  $x = 5b$ .

Let  $c = a - 2b$ .

$$x = 5x - 4x = 5(2a) - 4(5b) = 10a - 20b = 10(a - 2b) = 10c.$$

Therefore,  $\exists c \in \mathbb{Z}$ ,  $x = 10c$ . i.e., 10 divides  $x$ .

Therefore, if 2 divides  $x$  and 5 divides  $x$ , then 10 divides  $x$ .

QED

□

6. Prove  $\forall a, x, y \in \mathbb{Z}$ , if  $a$  divides  $x + y$  and  $a$  divides  $2x + y$ , then  $a$  divides  $x$  and  $a$  divides  $y$ .

*Proof.*

Let  $a, x, y \in \mathbb{Z}$ .

Assume  $a$  divides  $x + y$  and  $a$  divides  $2x + y$ .

Let  $s, t \in \mathbb{Z}$  with  $x + y = as$  and  $2x + y = at$ .

Let  $u = t - s$  and let  $v = 2s - t$ .

$$\text{Then } x = 2x + y - (x + y) = at - as = a(t - s) = au.$$

$$\text{And, } y = 2x + 2y - (2x + y) = 2as - at = a(2s - t) = av.$$

Therefore,  $a$  divides  $x$  and  $a$  divides  $y$ .

Therefore, if  $a$  divides  $x + y$  and  $a$  divides  $2x + y$ , then  $a$  divides  $x$  and  $a$  divides  $y$ .

QED

□

7. Using a proof by contradiction and the well-ordering property, prove  $\forall x \in \mathbb{Z}$ , if  $x$  is odd, then  $\forall n \in \mathbb{N}$ ,  $x^n$  is odd.

*Proof.*

Let  $x \in \mathbb{Z}$ .

Assume  $x$  is odd and  $\exists n \in \mathbb{N}$ ,  $x^n$  is not odd.

Let  $n \in \mathbb{N}$  be smallest with  $x^n$  not odd.

Since  $x^1$  is odd but  $x^n$  is not odd, we have  $n \neq 1$ . This means  $n - 1 \in \mathbb{N}$ .

Since  $n$  is smallest in  $\mathbb{N}$  with  $x^n$  not odd and  $n - 1 \in \mathbb{N}$ , we have that  $x^{n-1}$  is odd.

Since now  $x$  is odd and  $x^{n-1}$  is odd, let  $a, b \in \mathbb{Z}$  with  $x = 2a + 1$  and  $x^{n-1} = 2b + 1$ .

Let  $c = bx + a$ .

$$x^n = x(x^{n-1}) = x(2b + 1) = 2bx + x = 2bx + 2a + 1 = 2c + 1.$$

Therefore,  $x^n$  is odd, which is a contradiction, since  $x^n$  is not odd.

Therefore, if  $x$  is odd, then  $\forall n \in \mathbb{N}$ ,  $x^n$  is odd.

QED

□

8. Using a proof by contradiction and the well-ordering property, prove  $\forall x \in \mathbb{R}$ , if  $2 < x$ , then  $\forall n \in \mathbb{N}$ ,  $2^n < x^n$ .

*Proof.*

Let  $x \in \mathbb{R}$ .

Assume  $2 < x$  and  $\exists n \in \mathbb{N}$  with  $x^n \leq 2^n$ .

Let  $n \in \mathbb{N}$  be smallest with  $x^n \leq 2^n$ .

Since  $2^1 < x^1$  but  $x^n \leq 2^n$ , we have  $n \neq 1$ . This means  $n - 1 \in \mathbb{N}$ .

Note that since  $2 < x$ , we have  $0 < x$ , and so  $x^n(x^{-1}) \leq 2^n(x^{-1})$ . Then  $x^{n-1} \leq 2^n x^{-1}$ .

Also, since  $2 < x$ , we have  $x^{-1} < 2^{-1}$ , and so  $(2^n)x^{-1} < (2^n)2^{-1}$ . Then  $2^n x^{-1} < 2^{n-1}$ .

Since  $x^{n-1} \leq 2^n x^{-1}$  and  $2^n x^{-1} < 2^{n-1}$ , we have  $x^{n-1} \leq 2^{n-1}$ .

This contradicts  $n$  be the smallest natural number with this property.

Therefore, if  $2 < x$ , then  $\forall n \in \mathbb{N}$ ,  $2^n < x^n$ .

QED

□

9. Prove  $\forall x \in \mathbb{R}$ , if  $0 \leq x < 1$ , then  $\exists n \in \mathbb{N}$ ,  $\frac{n-1}{n} \leq x < \frac{n}{n+1}$ .

*Proof.*

Let  $x \in \mathbb{R}$ .

Assume  $0 < x < 1$ .

Since  $x < 1$ , we have  $0 < 1 - x$ .

By the Archimedean property,  $\exists n \in \mathbb{N}$ ,  $x < (1 - x)n$ .

Let  $n \in \mathbb{N}$  be smallest with  $x < (1 - x)n$ .

Then  $x < n - nx$ , and so  $x + nx < n$ . i.e.,  $x(n + 1) < n$ , giving us  $x < \frac{n}{n+1}$ .

Case 1:  $n = 1$ .

Since  $0 \leq x$ , we have  $n - 1 \leq x$ , and so  $\frac{n-1}{n} \leq x$ .

Case 2:  $1 < n$ .

In this case,  $0 < n - 1$ , and so  $n - 1 \in \mathbb{N}$ .

Since  $n$  is smallest in  $\mathbb{N}$  with  $x < (1 - x)n$ , we then have  $(1 - x)(n - 1) \leq x$ .

Then  $n - 1 - x(n - 1) \leq x$ , and so  $n - 1 \leq x + x(n - 1)$ .

This gives us  $n - 1 \leq nx$ , and so  $\frac{n-1}{n} \leq x$ .

Therefore,  $\exists n \in \mathbb{N}$ ,  $\frac{n-1}{n} \leq x < \frac{n}{n+1}$ .

QED

□

10. Using the principle of mathematical induction, prove  $\forall x \in \mathbb{Z}$ , if  $\exists a \in \mathbb{Z}$ ,  $x = 6a + 3$ , then  $\forall n \in \mathbb{N}$ ,  $\exists b \in \mathbb{Z}$ ,  $x^n = 6b + 3$ .

*Proof.*

Let  $x \in \mathbb{Z}$ , and assume  $\exists a \in \mathbb{Z}$ ,  $x = 6a + 3$ . Let  $a \in \mathbb{Z}$  with  $x = 6a + 3$ .

Let  $S = \{k \in \mathbb{N} \mid \exists b \in \mathbb{Z}, x^k = 6b + 3\}$ .

Since  $x^1 = x = 6a + 3$ , we have  $1 \in S$ .

Let  $n \in S$ .

Then  $\exists b \in \mathbb{Z}$ ,  $x^n = 6b + 3$ . Choose  $b \in \mathbb{Z}$  with  $x^n = 6b + 3$ .

Let  $c = 6ab + 3a + 3b + 1$ .

$x^{n+1} = x^n x = (6b + 3)(6a + 3) = 36ab + 18a + 18b + 9 = 36ab + 18a + 18b + 6 + 3$ .

Then  $x^{n+1} = 6(6ab + 3a + 3b + 1) + 3 = 6c + 3$ .

Thus,  $n + 1 \in S$ .

Therefore,  $S$  is inductive.

By the PMI,  $\forall n \in \mathbb{N}$ ,  $n \in S$ . i.e.,  $\forall n \in \mathbb{N}$ ,  $\exists b \in \mathbb{Z}$ ,  $x^n = 6b + 3$ .

QED

□

11. Using the principle of mathematical induction, prove  $\forall x \in \mathbb{Z}$ , if 3 divides  $x - 1$ , then  $\forall n \in \mathbb{N}$ , 3 divides  $x^n - 1$ .

*Proof.*

Let  $x \in \mathbb{Z}$ .

Assume 3 divides  $x - 1$

Let  $a \in \mathbb{Z}$  with  $x - 1 = 3a$ .

Let  $S = \{k \in \mathbb{N} \mid 3 \text{ divides } x^k - 1\}$ .

Since  $x^1 - 1 = x - 1 = 3a$ , we have  $1 \in S$ .

Let  $n \in S$ .

Let  $b \in \mathbb{Z}$  with  $x^n - 1 = 3b$ .

Let  $c = bx + a$ .

$$\begin{aligned} x^{n+1} - 1 &= x^{n+1} - x + x - 1 \\ &= (x^n - 1)x + x - 1 \\ &= 3bx + 3a \\ &= 3(bx + a) \\ &= 3c \end{aligned}$$

Thus, 3 divides  $x^{n+1} - 1$ .

Therefore,  $n + 1 \in S$ .

Therefore,  $S$  is inductive.

By the PMI,  $\forall n \in \mathbb{N}$ ,  $n \in S$ . i.e.,  $\forall n \in \mathbb{N}$ , 3 divides  $x^n - 1$ .

Therefore, if 3 divides  $x - 1$ , then  $\forall n \in \mathbb{N}$ , 3 divides  $x^n - 1$ .

QED

□

12. Using the principle of mathematical induction, prove  $\forall a, x, y \in \mathbb{Z}$ , if  $a$  divides  $x - y$ , then  $\forall n \in \mathbb{N}$ ,  $a$  divides  $x^n - y^n$ .

*Proof.*

Let  $a, x, y \in \mathbb{Z}$ .

Assume  $a$  divides  $x - y$

Let  $p \in \mathbb{Z}$  with  $x - y = ap$ .

Let  $S = \{k \in \mathbb{N} \mid a \text{ divides } x^k - y^k\}$ .

Since  $x^1 - y^1 = x - y = ap$ , we have  $1 \in S$ .

Let  $n \in S$ .

Let  $q \in \mathbb{Z}$  with  $x^n - y^n = aq$ .

Let  $r = qx + py^n$ .

$$\begin{aligned} x^{n+1} - y^{n+1} &= x^{n+1} - y^n x + y^n x - y^{n+1} \\ &= (x^n - y^n)x + y^n(x - y) \\ &= aqx + apy^n \\ &= a(qx + py^n) \\ &= ar \end{aligned}$$

Thus,  $a$  divides  $x^{n+1} - y^{n+1}$ .

Therefore,  $n + 1 \in S$ .

Therefore,  $S$  is inductive.

By the PMI,  $\forall n \in \mathbb{N}$ ,  $n \in S$ . i.e.,  $\forall n \in \mathbb{N}$ ,  $a$  divides  $x^n - y^n$ .

Therefore, if  $a$  divides  $x - y$ , then  $\forall n \in \mathbb{N}$ ,  $a$  divides  $x^n - y^n$ .

QED

□

13. Using the principle of mathematical induction, prove  $\forall x \in \mathbb{R}$ , if  $0 < x < 1$ , then  $\forall n \in \mathbb{N}$ ,  $x^n < 1$ .

*Proof.*

Let  $x \in \mathbb{R}$ .

Assume  $0 < x < 1$ .

Let  $S = \{k \in \mathbb{N} \mid x^k < 1\}$ .

Since  $x^1 < 1$  by our assumption, we have  $1 \in S$ .

Let  $n \in S$ .

Then  $x^n < 1$ .

Since  $0 < x$ , we have  $x^n(x) < 1(x)$ , and so  $x^{n+1} < x$ .

Now,  $x^{n+1} < x$  and  $x < 1$ , which gives us  $x^{n+1} < 1$ .

Therefore,  $n + 1 \in S$ .

Therefore,  $S$  is inductive.

By the PMI,  $\forall n \in \mathbb{N}$ ,  $n \in S$ . i.e.,  $\forall n \in \mathbb{N}$ ,  $x^n < 1$ .

Therefore, if  $0 < x < 1$ , then  $\forall n \in \mathbb{N}$ ,  $x^n < 1$ .

QED

□

14. Using the principle of mathematical induction, prove  $\forall n \in \mathbb{N}$ ,  $\sum_{k=1}^n 4k + 3 = 2n^2 + 5n$ .

*Proof.*

Let  $S = \{n \in \mathbb{N} \mid \sum_{k=1}^n 4k + 3 = 2n^2 + 5n\}$ .

$\sum_{k=1}^1 4k + 3 = 4(1) + 3 = 7 = 2 + 5 = 2(1)^2 + 5(1)$ .

Thus,  $1 \in S$ .

Let  $n \in S$ .

Then  $\sum_{k=1}^n 4k + 3 = 2n^2 + 5n$ .

$$\begin{aligned} \sum_{k=1}^{n+1} 4k + 3 &= \left( \sum_{k=1}^n 4k + 3 \right) + 4(n+1) + 3 \\ &= 2n^2 + 5n + 4(n+1) + 3 \\ &= 2n^2 + 4n + 7 + 5n \\ &= 2n^2 + 4n + 2 + 5 + 5n \\ &= 2(n^2 + 2n + 1) + 5(n+1) \\ &= 2(n+1)^2 + 5(n+1) \end{aligned}$$

Thus,  $n + 1 \in S$ .

Therefore,  $S$  is inductive.

By the PMI,  $\forall n \in \mathbb{N}$ ,  $n \in S$ .

QED

□

15. Using the principle of mathematical induction, prove  $\forall n \in \mathbb{N}, \sum_{k=1}^n \frac{1}{2^k} = 1 - \frac{1}{2^n}$ .

*Proof.*

Let  $S = \{n \in \mathbb{N} \mid \sum_{k=1}^n \frac{1}{2^k} = 1 - \frac{1}{2^n}\}$ .

$$\sum_{k=1}^1 \frac{1}{2^k} = \frac{1}{2^1} = \frac{1}{2} = 1 - \frac{1}{2} = 1 - \frac{1}{2^1}.$$

Thus,  $1 \in S$ .

Let  $n \in S$ .

$$\text{Then } \sum_{k=1}^n \frac{1}{2^k} = 1 - \frac{1}{2^n}.$$

$$\begin{aligned} \sum_{k=1}^{n+1} \frac{1}{2^k} &= \left( \sum_{k=1}^n \frac{1}{2^k} \right) + \frac{1}{2^{n+1}} \\ &= 1 - \frac{1}{2^n} + \frac{1}{2^{n+1}} \\ &= 1 - \frac{2}{2^{n+1}} + \frac{1}{2^{n+1}} \\ &= 1 - \frac{1}{2^{n+1}} \end{aligned}$$

Thus,  $n+1 \in S$ .

Therefore,  $S$  is inductive.

By the PMI,  $\forall n \in \mathbb{N}, n \in S$ .

QED

□

16. Prove  $\forall a, b \in \mathbb{R}$ , if  $a < b$ , then  $(-\infty, b) \setminus (-\infty, a) = [a, b)$ .

*Proof.*

Let  $a, b \in \mathbb{R}$ .

Assume  $a < b$ .

Let  $x \in \mathbb{R}$  and assume  $x \in (-\infty, b) \setminus (-\infty, a)$ .

Then  $x \in (-\infty, b)$ , so  $x < b$ , and  $x \notin (-\infty, a)$ , so  $a \leq x$ .

Since  $a \leq x$  and  $x < b$ , we have  $x \in [a, b)$ .

Therefore,  $\forall x \in \mathbb{R}$ , if  $x \in (-\infty, b) \setminus (-\infty, a)$ , then  $x \in [a, b)$ .

Thus,  $(-\infty, b) \setminus (-\infty, a) \subseteq [a, b)$ .

Conversely, let  $x \in \mathbb{R}$  and assume  $x \in [a, b)$ .

Then  $a \leq x$  and  $x < b$ .

Since  $a \leq x$ , we have  $x \notin (-\infty, a)$ .

Since  $x < b$ , we have  $x \in (-\infty, b)$ .

Now,  $x \in (-\infty, b)$  and  $x \notin (-\infty, a)$ , so  $x \in (-\infty, b) \setminus (-\infty, a)$ .

Therefore,  $[a, b) \subseteq (-\infty, b) \setminus (-\infty, a)$ .

Therefore,  $(-\infty, b) \setminus (-\infty, a) = [a, b)$ .

Therefore, if  $a < b$ , then  $(-\infty, b) \setminus (-\infty, a) = [a, b)$ .

Therefore,  $\forall a, b \in \mathbb{R}$ , if  $a < b$ , then  $(-\infty, b) \setminus (-\infty, a) = [a, b)$ .

□

17. Prove  $(-\infty, 3] \setminus (1, 2) = (-\infty, 1] \cup [2, 3]$ .

*Proof.*

Let  $x \in \mathbb{R}$  and assume  $x \in (-\infty, 3] \setminus (1, 2)$ .

Then  $x \in (-\infty, 3]$ , so  $x \leq 3$ , and  $x \notin (1, 2)$ , so either  $x \leq 1$  or  $2 \leq x$ .

Case 1:  $x \leq 1$ .

In this case, we have  $x \in (-\infty, 1]$ , so  $x \in (-\infty, 1] \cup [2, 3]$ .

Case 2:  $2 \leq x$ .

Now,  $2 \leq x$  and  $x \leq 3$ , so  $x \in [2, 3]$ .

This implies that  $x \in (-\infty, 1] \cup [2, 3]$ .

Therefore,  $(-\infty, 3] \setminus (1, 2) \subseteq (-\infty, 1] \cup [2, 3]$ .

Conversely, let  $x \in \mathbb{R}$  and assume  $x \in (-\infty, 1] \cup [2, 3]$ .

Then  $x \in (-\infty, 1]$  or  $x \in [2, 3]$ .

Case 1:  $x \in (-\infty, 1]$ .

In this case,  $x \leq 1$ , so  $x \notin (1, 2)$ .

Also, since  $x \leq 1$  and  $1 \leq 3$ , we have  $x \leq 3$ , so  $x \in (-\infty, 3]$ .

Now,  $x \in (-\infty, 3]$  and  $x \notin (1, 2)$ , so  $x \in (-\infty, 3] \setminus (1, 2)$ .

Case 2:  $x \in [2, 3]$ .

In this case,  $2 \leq x$ , so  $x \notin (1, 2)$ , and  $x \leq 3$ , so  $x \in (-\infty, 3]$ .

Again, we have  $x \in (-\infty, 3]$  and  $x \notin (1, 2)$ , so  $x \in (-\infty, 3] \setminus (1, 2)$ .

Therefore,  $(-\infty, 1] \cup [2, 3] \subseteq (-\infty, 3] \setminus (1, 2)$ .

Therefore,  $(-\infty, 3] \setminus (1, 2) = (-\infty, 1] \cup [2, 3]$ . □

18. Prove  $\langle 5 \rangle \cap \langle 4 \rangle = \langle 20 \rangle$ .

*Proof.*

Let  $x \in \mathbb{Z}$  and assume  $x \in \langle 5 \rangle \cap \langle 4 \rangle$ .

Then  $x \in \langle 5 \rangle$  and  $x \in \langle 4 \rangle$ .

Choose  $a, b \in \mathbb{Z}$  with  $x = 5a$  and  $x = 4b$ .

Put  $c = b - a$ .

$$x = 5x - 4x = 5(4b) - 4(5a) = 20b - 20a = 20c.$$

Therefore,  $\exists c \in \mathbb{Z}$ ,  $x = 20c$ .

Thus,  $x \in \langle 20 \rangle$ .

Therefore,  $\langle 5 \rangle \cap \langle 4 \rangle \subseteq \langle 20 \rangle$ .

Conversely, let  $x \in \mathbb{Z}$  and assume  $x \in \langle 20 \rangle$ .

Accordingly, choose  $q \in \mathbb{Z}$  with  $x = 20q$ .

Put  $s = 4q$ .

$$\text{Then } x = 20q = 5(4q) = 5s.$$

Therefore,  $\exists s \in \mathbb{Z}$ ,  $x = 5s$ , which means  $x \in \langle 5 \rangle$ .

Put  $t = 5q$ .

$$x = 20q = 4(5q) = 4t.$$

Therefore,  $\exists t \in \mathbb{Z}$ ,  $x = 4t$ . Thus,  $x \in \langle 4 \rangle$ .

We now have  $x \in \langle 5 \rangle$  and  $x \in \langle 4 \rangle$ , which means  $x \in \langle 5 \rangle \cap \langle 4 \rangle$ .

Therefore,  $\langle 20 \rangle \subseteq \langle 5 \rangle \cap \langle 4 \rangle$ .

Therefore,  $\langle 5 \rangle \cap \langle 4 \rangle = \langle 20 \rangle$ . □

19. Prove  $\forall m, n \in \mathbb{Z}$ , if  $m$  divides  $n$ , then  $n + \langle m \rangle = \langle m \rangle$ .

*Proof.*

Let  $m, n \in \mathbb{Z}$ .

Assume  $m$  divides  $n$ .

Choose  $q \in \mathbb{Z}$  with  $n = mq$ .

Let  $x \in n + \langle m \rangle$ .

Choose  $a \in \mathbb{Z}$  with  $x = n + ma$ .

Let  $b = q + a$ .

Now,  $x = n + ma = mq + ma = m(q + a) = mb$ .

This proves  $x \in \langle m \rangle$ .

Thus,  $n + \langle m \rangle \subseteq \langle m \rangle$ .

Conversely, let  $x \in \langle m \rangle$ .

Choose  $u \in \mathbb{Z}$  with  $x = mu$ .

Let  $v = u - q$ .

Now,  $x = mu = n + mu - n = n + mu - mq = n + m(u - q) = n + mv$ .

This proves  $x \in n + \langle m \rangle$ .

Thus,  $\langle m \rangle \subseteq n + \langle m \rangle$ .

Therefore,  $n + \langle m \rangle = \langle m \rangle$ .

Therefore, if  $m$  divides  $n$ , then  $n + \langle m \rangle = \langle m \rangle$ .

QED. □

20. Prove  $\langle 10 \rangle + \langle 15 \rangle = \langle 5 \rangle$ .

*Proof.*

Let  $x \in \langle 10 \rangle + \langle 15 \rangle$ .

Choose  $a, b \in \mathbb{Z}$  with  $x = 10a + 15b$ .

Let  $c = 2a + 3b$ .

Now,  $x = 10a + 15b = 5(2a + 3b) = 5c$ .

Thus,  $x \in \langle 5 \rangle$ .

Therefore,  $\langle 10 \rangle + \langle 15 \rangle \subseteq \langle 5 \rangle$ .

Conversely, let  $x \in \langle 5 \rangle$ .

Choose  $u \in \mathbb{Z}$  with  $x = 5u$ .

Let  $v = -u$ .

Now,  $x = 5u = -10u + 15u = 10v + 15u$ .

This proves  $x \in \langle 10 \rangle + \langle 15 \rangle$ .

Therefore,  $\langle 5 \rangle \subseteq \langle 10 \rangle + \langle 15 \rangle$ .

QED. □